theories/Sep/Hoare.v
@@ -69,163 +69,161 @@ Module ProgramLogic.
                  (asn.interpret ens ι -∗ post)) ->
         LTriple δΔ pre post (MkLemma _ _ θΔ req ens).
 
-    Reserved Notation "# f ⦃ P ⦄ s ; δ ⦃ Q ⦄".
+    Reserved Notation "⦃ P ⦄ s ; δ ⦃ Q ⦄".
 
     Inductive Triple {Γ : PCtx} (δ : CStore Γ) {τ : Ty} :
-      forall (fuel : nat) (pre : L) (s : Stm Γ τ) (post :  Val τ -> CStore Γ -> L), Prop :=
+      forall  (pre : L) (s : Stm Γ τ) (post :  Val τ -> CStore Γ -> L), Prop :=
     | rule_consequence
-        {fuel : nat} {s : Stm Γ τ} {P P' : L} {Q Q' : Val τ -> CStore Γ -> L}
+        {s : Stm Γ τ} {P P' : L} {Q Q' : Val τ -> CStore Γ -> L}
         (Hleft : P ⊢ P') (Hright : forall v δ', Q' v δ' ⊢ Q v δ') :
-        # fuel ⦃ P' ⦄ s ; δ ⦃ Q' ⦄ ->
-        # fuel ⦃ P ⦄ s ; δ ⦃ Q ⦄
+        ⦃ P' ⦄ s ; δ ⦃ Q' ⦄ ->
+        ⦃ P ⦄ s ; δ ⦃ Q ⦄
     | rule_frame
-        {fuel : nat } (s : Stm Γ τ) (R P : L) (Q : Val τ -> CStore Γ -> L) :
-        # fuel ⦃ P ⦄ s ; δ ⦃ Q ⦄ ->
-        # fuel ⦃ R ∗ P ⦄ s ; δ ⦃ fun v δ' => R ∗ Q v δ' ⦄
+        (s : Stm Γ τ) (R P : L) (Q : Val τ -> CStore Γ -> L) :
+        ⦃ P ⦄ s ; δ ⦃ Q ⦄ ->
+        ⦃ R ∗ P ⦄ s ; δ ⦃ fun v δ' => R ∗ Q v δ' ⦄
     | rule_pull
-        {fuel : nat} (s : Stm Γ τ) (P : L) (Q : Prop) (R : Val τ -> CStore Γ -> L) :
-        (Q -> # fuel ⦃ P ⦄ s ; δ ⦃ R ⦄) ->
-        # fuel ⦃ P ∧ ⌜Q⌝ ⦄ s ; δ ⦃ R ⦄
+        (s : Stm Γ τ) (P : L) (Q : Prop) (R : Val τ -> CStore Γ -> L) :
+        (Q -> ⦃ P ⦄ s ; δ ⦃ R ⦄) ->
+        ⦃ P ∧ ⌜Q⌝ ⦄ s ; δ ⦃ R ⦄
     | rule_exist
-        {fuel : nat} (s : Stm Γ τ) {A : Type} {P : A -> L} {Q : Val τ -> CStore Γ -> L} :
-        (forall x, # fuel ⦃ P x ⦄ s ; δ ⦃ Q ⦄) ->
-        # fuel ⦃ ∃ x, P x ⦄ s ; δ ⦃ Q ⦄
+        (s : Stm Γ τ) {A : Type} {P : A -> L} {Q : Val τ -> CStore Γ -> L} :
+        (forall x, ⦃ P x ⦄ s ; δ ⦃ Q ⦄) ->
+        ⦃ ∃ x, P x ⦄ s ; δ ⦃ Q ⦄
     | rule_stm_val
-        {fuel : nat} {l : Val τ} {P : L} {Q : Val τ -> CStore Γ -> L} :
+        {l : Val τ} {P : L} {Q : Val τ -> CStore Γ -> L} :
         (P ⊢ Q l δ) ->
-        # fuel ⦃ P ⦄ stm_val τ l ; δ ⦃ Q ⦄
+        ⦃ P ⦄ stm_val τ l ; δ ⦃ Q ⦄
     | rule_stm_exp
-        {fuel : nat} {e : Exp Γ τ} {P : L} {Q : Val τ -> CStore Γ -> L} :
+        {e : Exp Γ τ} {P : L} {Q : Val τ -> CStore Γ -> L} :
         (P ⊢ Q (eval e δ) δ) ->
-        # fuel ⦃ P ⦄ stm_exp e ; δ ⦃ Q ⦄
+        ⦃ P ⦄ stm_exp e ; δ ⦃ Q ⦄
     | rule_stm_let
-        {fuel : nat} (x : PVar) (σ : Ty) (s : Stm Γ σ) (k : Stm (Γ ▻ x∷σ) τ)
+        (x : PVar) (σ : Ty) (s : Stm Γ σ) (k : Stm (Γ ▻ x∷σ) τ)
         (P : L) (Q : Val σ -> CStore Γ -> L)
         (R : Val τ -> CStore Γ -> L) :
-        # fuel ⦃ P ⦄ s ; δ ⦃ Q ⦄ ->
+        ⦃ P ⦄ s ; δ ⦃ Q ⦄ ->
         (forall (v : Val σ) (δ' : CStore Γ),
-            # fuel ⦃ Q v δ' ⦄ k ; env.snoc δ' (x∷σ) v ⦃ fun v δ'' => R v (env.tail δ'') ⦄ ) ->
-        # fuel ⦃ P ⦄ let: x := s in k ; δ ⦃ R ⦄
+            ⦃ Q v δ' ⦄ k ; env.snoc δ' (x∷σ) v ⦃ fun v δ'' => R v (env.tail δ'') ⦄ ) ->
+        ⦃ P ⦄ let: x := s in k ; δ ⦃ R ⦄
     | rule_stm_block
-        {fuel : nat} (Δ : PCtx) (δΔ : CStore Δ)
+        (Δ : PCtx) (δΔ : CStore Δ)
         (k : Stm (Γ ▻▻ Δ) τ)
         (P : L) (R : Val τ -> CStore Γ -> L) :
-        # fuel ⦃ P ⦄ k ; δ ►► δΔ ⦃ fun v δ'' => R v (env.drop Δ δ'') ⦄ ->
-        # fuel ⦃ P ⦄ stm_block δΔ k ; δ ⦃ R ⦄
+        ⦃ P ⦄ k ; δ ►► δΔ ⦃ fun v δ'' => R v (env.drop Δ δ'') ⦄ ->
+        ⦃ P ⦄ stm_block δΔ k ; δ ⦃ R ⦄
     | rule_stm_seq
-        {fuel : nat}
         (σ : Ty) (s1 : Stm Γ σ) (s2 : Stm Γ τ)
         (P : L) (Q : Val σ -> CStore Γ -> L) (R : Val τ -> CStore Γ -> L) :
-        # fuel ⦃ P ⦄ s1 ; δ ⦃ Q ⦄ ->
-        (forall v δ', # fuel ⦃ Q v δ' ⦄ s2 ; δ' ⦃ R ⦄) ->
-        # fuel ⦃ P ⦄ s1 ;; s2 ; δ ⦃ R ⦄
+        ⦃ P ⦄ s1 ; δ ⦃ Q ⦄ ->
+        (forall v δ', ⦃ Q v δ' ⦄ s2 ; δ' ⦃ R ⦄) ->
+        ⦃ P ⦄ s1 ;; s2 ; δ ⦃ R ⦄
     | rule_stm_assert
-        {fuel : nat} (e1 : Exp Γ ty.bool) (e2 : Exp Γ ty.string) (k : Stm Γ τ)
+        (e1 : Exp Γ ty.bool) (e2 : Exp Γ ty.string) (k : Stm Γ τ)
         (P : L) (Q : Val τ -> CStore Γ -> L) :
-        (eval e1 δ = true -> # fuel ⦃ P ⦄ k ; δ ⦃ Q ⦄) ->
-        # fuel ⦃ P ⦄ stm_assertk e1 e2 k ; δ ⦃ Q ⦄
+        (eval e1 δ = true -> ⦃ P ⦄ k ; δ ⦃ Q ⦄) ->
+        ⦃ P ⦄ stm_assertk e1 e2 k ; δ ⦃ Q ⦄
     | rule_stm_fail
-        {fuel : nat} (s : Val ty.string) (Q : Val τ -> CStore Γ -> L) :
-        # fuel ⦃ True ⦄ stm_fail τ s ; δ ⦃ Q ⦄
+        (s : Val ty.string) (Q : Val τ -> CStore Γ -> L) :
+        ⦃ True ⦄ stm_fail τ s ; δ ⦃ Q ⦄
     | rule_stm_read_register
-        {fuel : nat} (r : 𝑹𝑬𝑮 τ) (v : Val τ) :
-        # fuel ⦃ lptsreg r v ⦄
+        (r : 𝑹𝑬𝑮 τ) (v : Val τ) :
+        ⦃ lptsreg r v ⦄
           stm_read_register r ; δ
         ⦃ fun v' δ' => ⌜δ' = δ⌝ ∧ ⌜v' = v⌝ ∧ lptsreg r v ⦄
     | rule_stm_write_register
-        {fuel : nat} (r : 𝑹𝑬𝑮 τ) (w : Exp Γ τ) (v : Val τ)
+        (r : 𝑹𝑬𝑮 τ) (w : Exp Γ τ) (v : Val τ)
         (Q : Val τ -> CStore Γ -> L) :
-        # fuel ⦃ lptsreg r v ⦄
+        ⦃ lptsreg r v ⦄
           stm_write_register r w ; δ
         ⦃ fun v' δ' => ⌜δ' = δ⌝ ∧ ⌜v' = eval w δ⌝ ∧ lptsreg r v' ⦄
     | rule_stm_assign
-        {fuel : nat} (x : PVar) (xIn : (x∷τ ∈ Γ)%katamaran) (s : Stm Γ τ)
+        (x : PVar) (xIn : (x∷τ ∈ Γ)%katamaran) (s : Stm Γ τ)
         (P : L) (R : Val τ -> CStore Γ -> L) :
-        # fuel ⦃ P ⦄ s ; δ ⦃ fun v δ' => R v (δ' ⟪ x ↦ v ⟫)%env ⦄ ->
-        # fuel ⦃ P ⦄ stm_assign x s ; δ ⦃ R ⦄
+        ⦃ P ⦄ s ; δ ⦃ fun v δ' => R v (δ' ⟪ x ↦ v ⟫)%env ⦄ ->
+        ⦃ P ⦄ stm_assign x s ; δ ⦃ R ⦄
     | rule_stm_call
-        {fuel : nat} {Δ} {f : 𝑭 Δ τ} {es : NamedEnv (Exp Γ) Δ} {c : SepContract Δ τ}
+        {Δ} {f : 𝑭 Δ τ} {es : NamedEnv (Exp Γ) Δ} {c : SepContract Δ τ}
         (P : L) (Q : Val τ -> CStore Γ -> L) :
         CEnv f = Some c ->
         CTriple P c (evals es δ) (fun v => Q v δ) ->
-        # fuel ⦃ P ⦄ stm_call f es ; δ ⦃ Q ⦄
+        ⦃ P ⦄ stm_call f es ; δ ⦃ Q ⦄
     | rule_stm_call_inline
-        {fuel : nat} {Δ} (f : 𝑭 Δ τ) (es : NamedEnv (Exp Γ) Δ)
+        {Δ} (f : 𝑭 Δ τ) (es : NamedEnv (Exp Γ) Δ)
         (P : L) (Q : Val τ -> CStore Γ -> L) :
-        # fuel ⦃ P ⦄ FunDef f ; evals es δ ⦃ fun v _ => Q v δ ⦄ ->
-        # S fuel ⦃ P ⦄ stm_call f es ; δ ⦃ Q ⦄
+        ⦃ P ⦄ FunDef f ; evals es δ ⦃ fun v _ => Q v δ ⦄ ->
+        ⦃ P ⦄ stm_call f es ; δ ⦃ Q ⦄
     | rule_stm_call_frame (* TODO: remove stm_call_frame (similar for bind and block then) *)
-        {fuel : nat} (Δ : PCtx) (δΔ : CStore Δ) (s : Stm Δ τ)
+        (Δ : PCtx) (δΔ : CStore Δ) (s : Stm Δ τ)
         (P : L) (Q : Val τ -> CStore Γ -> L) :
-        # fuel ⦃ P ⦄ s ; δΔ ⦃ fun v _ => Q v δ ⦄ ->
-        # fuel ⦃ P ⦄ stm_call_frame δΔ s ; δ ⦃ Q ⦄ (* TODO: to S or not to S for the fuel *)
+        ⦃ P ⦄ s ; δΔ ⦃ fun v _ => Q v δ ⦄ ->
+        ⦃ P ⦄ stm_call_frame δΔ s ; δ ⦃ Q ⦄ (* TODO: to S or not to S for the fuel *)
     | rule_stm_foreign
-        {fuel : nat} {Δ} {f : 𝑭𝑿 Δ τ} (es : NamedEnv (Exp Γ) Δ)
+        {Δ} {f : 𝑭𝑿 Δ τ} (es : NamedEnv (Exp Γ) Δ)
         (P : L) (Q : Val τ -> CStore Γ -> L) :
         CTriple P (CEnvEx f) (evals es δ) (fun v => Q v δ) ->
-        # fuel ⦃ P ⦄ stm_foreign f es ; δ ⦃ Q ⦄
+        ⦃ P ⦄ stm_foreign f es ; δ ⦃ Q ⦄
     | rule_stm_lemmak
-        {fuel : nat} {Δ} {l : 𝑳 Δ} (es : NamedEnv (Exp Γ) Δ) (k : Stm Γ τ)
+        {Δ} {l : 𝑳 Δ} (es : NamedEnv (Exp Γ) Δ) (k : Stm Γ τ)
         (P Q : L) (R : Val τ -> CStore Γ -> L) :
         LTriple (evals es δ) P Q (LEnv l) ->
-        # fuel ⦃ Q ⦄ k ; δ ⦃ R ⦄ ->
-        # fuel ⦃ P ⦄ stm_lemmak l es k ; δ ⦃ R ⦄
+        ⦃ Q ⦄ k ; δ ⦃ R ⦄ ->
+        ⦃ P ⦄ stm_lemmak l es k ; δ ⦃ R ⦄
     | rule_stm_bind
-        {fuel : nat} {σ : Ty} (s : Stm Γ σ) (k : Val σ -> Stm Γ τ)
+        {σ : Ty} (s : Stm Γ σ) (k : Val σ -> Stm Γ τ)
         (P : L) (Q : Val σ -> CStore Γ -> L)
         (R : Val τ -> CStore Γ -> L) :
-        # fuel ⦃ P ⦄ s ; δ ⦃ Q ⦄ ->
+        ⦃ P ⦄ s ; δ ⦃ Q ⦄ ->
         (forall (v__σ : Val σ) (δ' : CStore Γ),
-           # fuel ⦃ Q v__σ δ' ⦄ k v__σ ; δ' ⦃ R ⦄) ->
-        # fuel ⦃ P ⦄ stm_bind s k ; δ ⦃ R ⦄
+           ⦃ Q v__σ δ' ⦄ k v__σ ; δ' ⦃ R ⦄) ->
+        ⦃ P ⦄ stm_bind s k ; δ ⦃ R ⦄
     | rule_stm_debugk
-        {fuel : nat} (k : Stm Γ τ)
+        (k : Stm Γ τ)
         (P : L) (Q : Val τ -> CStore Γ -> L) :
-        # fuel ⦃ P ⦄ k ; δ ⦃ Q ⦄ ->
-        # fuel ⦃ P ⦄ stm_debugk k ; δ ⦃ Q ⦄
-
+        ⦃ P ⦄ k ; δ ⦃ Q ⦄ ->
+        ⦃ P ⦄ stm_debugk k ; δ ⦃ Q ⦄
     | rule_stm_pattern_match
-        {fuel : nat} {σ} (s : Stm Γ σ) (pat : Pattern σ)
+        {σ} (s : Stm Γ σ) (pat : Pattern σ)
         (rhs : forall (pc : PatternCase pat), Stm (Γ ▻▻ PatternCaseCtx pc) τ)
         (P : L) (Q : Val σ -> CStore Γ -> L) (R : Val τ -> CStore Γ -> L) :
-        # fuel ⦃ P ⦄ s ; δ ⦃ Q ⦄ ->
+        ⦃ P ⦄ s ; δ ⦃ Q ⦄ ->
         (forall pc δpc δ',
-           # fuel ⦃ Q (pattern_match_val_reverse pat pc δpc) δ' ⦄ rhs pc ; δ' ►► δpc
+           ⦃ Q (pattern_match_val_reverse pat pc δpc) δ' ⦄ rhs pc ; δ' ►► δpc
            ⦃ fun v2 δ' => R v2 (env.drop (PatternCaseCtx pc) δ') ⦄) ->
-        # fuel ⦃ P ⦄ stm_pattern_match s pat rhs ; δ ⦃ R ⦄
+        ⦃ P ⦄ stm_pattern_match s pat rhs ; δ ⦃ R ⦄
 
-    where "# f ⦃ P ⦄ s ; δ ⦃ Q ⦄" := (@Triple _ δ _ f P%I s Q%I).
+    where "⦃ P ⦄ s ; δ ⦃ Q ⦄" := (@Triple _ δ _ P%I s Q%I).
 
-    Notation "# f ⦃ P ⦄ s ; δ ⦃ Q ⦄" := (@Triple _ δ _ f P%I s Q%I).
+    Notation "⦃ P ⦄ s ; δ ⦃ Q ⦄" := (@Triple _ δ _ P%I s Q%I).
 
-    Lemma rule_consequence_left {Γ σ} {fuel : nat} {δ : CStore Γ} {s : Stm Γ σ}
+    Lemma rule_consequence_left {Γ σ} {δ : CStore Γ} {s : Stm Γ σ}
       (P1 : L) {P2 : L} {Q : Val σ -> CStore Γ -> L} :
-      # fuel ⦃ P1 ⦄ s ; δ ⦃ Q ⦄ -> (P2 ⊢ P1) -> # fuel ⦃ P2 ⦄ s ; δ ⦃ Q ⦄.
+      ⦃ P1 ⦄ s ; δ ⦃ Q ⦄ -> (P2 ⊢ P1) -> ⦃ P2 ⦄ s ; δ ⦃ Q ⦄.
     Proof.
       intros H hyp. exact (rule_consequence δ hyp (fun _ _ => reflexivity _) H).
     Qed.
 
-    Lemma rule_consequence_right {Γ σ} {fuel : nat} {δ : CStore Γ} {s : Stm Γ σ}
+    Lemma rule_consequence_right {Γ σ} {δ : CStore Γ} {s : Stm Γ σ}
       {P : L} Q {Q'} :
-      # fuel ⦃ P ⦄ s ; δ ⦃ Q ⦄ -> (forall v δ, Q v δ ⊢ Q' v δ) -> # fuel ⦃ P ⦄ s ; δ ⦃ Q' ⦄.
+      ⦃ P ⦄ s ; δ ⦃ Q ⦄ -> (forall v δ, Q v δ ⊢ Q' v δ) -> ⦃ P ⦄ s ; δ ⦃ Q' ⦄.
     Proof.
       intros H hyp. exact (rule_consequence δ (reflexivity P) hyp H).
     Qed.
 
-    Lemma rule_exist' {Γ : PCtx} {δ : CStore Γ} {fuel : nat} {A : Type} {σ : Ty} (s : Stm Γ σ)
+    Lemma rule_exist' {Γ : PCtx} {δ : CStore Γ} {A : Type} {σ : Ty} (s : Stm Γ σ)
       {P : A -> L} (Q :  A -> Val σ -> CStore Γ -> L) :
-      (forall x, # fuel ⦃ P x ⦄ s ; δ ⦃ Q x ⦄) ->
-      # fuel ⦃ ∃ x, P x ⦄ s ; δ ⦃ fun v δ' => ∃ x, Q x v δ' ⦄.
+      (forall x, ⦃ P x ⦄ s ; δ ⦃ Q x ⦄) ->
+      ⦃ ∃ x, P x ⦄ s ; δ ⦃ fun v δ' => ∃ x, Q x v δ' ⦄.
     Proof.
       intros hyp. apply rule_exist. intros x.
       apply (rule_consequence_right (Q x) (hyp x)).
       intros v δ'. now apply bi.exist_intro' with x.
     Qed.
 
-    Lemma rule_disj {Γ σ} {fuel : nat} {δ : CStore Γ} {s : Stm Γ σ}
+    Lemma rule_disj {Γ σ} {δ : CStore Γ} {s : Stm Γ σ}
       {P Q : L} {R : Val σ -> CStore Γ -> L} :
-      # fuel ⦃ P ⦄ s ; δ ⦃ R ⦄ -> # fuel ⦃ Q ⦄ s ; δ ⦃ R ⦄ ->
-      # fuel ⦃ P ∨ Q ⦄ s ; δ ⦃ R ⦄.
+      ⦃ P ⦄ s ; δ ⦃ R ⦄ -> ⦃ Q ⦄ s ; δ ⦃ R ⦄ ->
+      ⦃ P ∨ Q ⦄ s ; δ ⦃ R ⦄.
     Proof.
       intros H1 H2.
       apply (rule_consequence_left (∃ b : bool, if b then P else Q)).
@@ -235,10 +233,10 @@ Module ProgramLogic.
         + now apply bi.exist_intro' with false.
     Qed.
 
-    Lemma rule_disj' {Γ σ} {fuel : nat} {δ : CStore Γ} {s : Stm Γ σ}
+    Lemma rule_disj' {Γ σ} {δ : CStore Γ} {s : Stm Γ σ}
       {P1 P2 : L} {Q1 Q2 : Val σ -> CStore Γ -> L} :
-      # fuel ⦃ P1 ⦄ s ; δ ⦃ Q1 ⦄ -> # fuel ⦃ P2 ⦄ s ; δ ⦃ Q2 ⦄ ->
-      # fuel ⦃ P1 ∨ P2 ⦄ s ; δ ⦃ fun v δ' => Q1 v δ' ∨ Q2 v δ' ⦄.
+      ⦃ P1 ⦄ s ; δ ⦃ Q1 ⦄ -> ⦃ P2 ⦄ s ; δ ⦃ Q2 ⦄ ->
+      ⦃ P1 ∨ P2 ⦄ s ; δ ⦃ fun v δ' => Q1 v δ' ∨ Q2 v δ' ⦄.
     Proof.
       intros H1 H2.
       apply rule_disj.
@@ -248,61 +246,31 @@ Module ProgramLogic.
         intros ? ?. apply bi.or_intro_r.
     Qed.
 
-    Lemma rule_false {Γ σ} {fuel : nat} {δ : CStore Γ} {s : Stm Γ σ}
+    Lemma rule_false {Γ σ} {δ : CStore Γ} {s : Stm Γ σ}
       {Q : Val σ -> CStore Γ -> L} :
-      # fuel ⦃ False ⦄ s ; δ ⦃ Q ⦄.
+      ⦃ False ⦄ s ; δ ⦃ Q ⦄.
     Proof.
       apply (rule_consequence_left (∃ (x : Empty_set), True)).
       - apply rule_exist; intros [].
       - auto.
     Qed.
 
+    Definition WP {Γ τ} (s : Stm Γ τ) (POST :  Val τ -> CStore Γ -> L) : CStore Γ -> L :=
+      fun δ => (∃ (P : L), P ∧ ⌜⦃ P ⦄ s; δ ⦃ POST ⦄⌝)%I.
 
-    Lemma rule_S_fuel {Γ σ} {fuel : nat} {δ : CStore Γ} {s : Stm Γ σ} {P Q} :
-      # fuel ⦃ P ⦄ s ; δ ⦃ Q ⦄ →
-      # S fuel ⦃ P ⦄ s ; δ ⦃ Q ⦄.
-    Proof.
-      intros H. induction H.
-      - by eapply rule_consequence.
-      - by eapply rule_frame.
-      - by eapply rule_pull.
-      - by eapply rule_exist.
-      - by apply rule_stm_val.
-      - by apply rule_stm_exp.
-      - by eapply rule_stm_let.
-      - by apply rule_stm_block.
-      - by eapply rule_stm_seq.
-      - by apply rule_stm_assert.
-      - by apply rule_stm_fail.
-      - by apply rule_stm_read_register.
-      - by apply rule_stm_write_register.
-      - by apply rule_stm_assign.
-      - by eapply rule_stm_call.
-      - by apply rule_stm_call_inline.
-      - by apply rule_stm_call_frame.
-      - by apply rule_stm_foreign.
-      - by eapply rule_stm_lemmak.
-      - by eapply rule_stm_bind.
-      - by apply rule_stm_debugk.
-      - by eapply rule_stm_pattern_match.
-    Qed.
-
-    Definition WP {Γ τ} (fuel : nat) (s : Stm Γ τ) (POST :  Val τ -> CStore Γ -> L) : CStore Γ -> L :=
-      fun δ => (∃ (P : L), P ∧ ⌜# fuel ⦃ P ⦄ s; δ ⦃ POST ⦄⌝)%I.
-
-    Lemma rule_wp {Γ σ} (fuel : nat) (s : Stm Γ σ) (POST :  Val σ -> CStore Γ -> L) (δ : CStore Γ) :
-      # fuel ⦃ WP fuel s POST δ ⦄ s ; δ ⦃ POST ⦄.
+    Lemma rule_wp {Γ σ} (s : Stm Γ σ) (POST :  Val σ -> CStore Γ -> L) (δ : CStore Γ) :
+      ⦃ WP s POST δ ⦄ s ; δ ⦃ POST ⦄.
     Proof. apply rule_exist; intros P; now apply rule_pull. Qed.
 
-    #[export] Instance proper_triple_entails {Γ δ τ f} :
-      Proper (Basics.flip (⊢) ==> eq ==> pointwise_relation _ (pointwise_relation _ (⊢)) ==> Basics.impl) (@Triple Γ δ τ f).
+    #[export] Instance proper_triple_entails {Γ δ τ} :
+      Proper (Basics.flip (⊢) ==> eq ==> pointwise_relation _ (pointwise_relation _ (⊢)) ==> Basics.impl) (@Triple Γ δ τ).
     Proof.
       intros P Q qp s s' eq__s R S rs H; subst s'.
       eapply rule_consequence. apply qp. apply rs. apply H.
     Qed.
 
-    #[export] Instance proper_triple_equiv {Γ δ τ f} :
-      Proper ((⊣⊢) ==> eq ==> pointwise_relation _ (pointwise_relation _ (⊣⊢)) ==> iff) (@Triple Γ δ τ f).
+    #[export] Instance proper_triple_equiv {Γ δ τ} :
+      Proper ((⊣⊢) ==> eq ==> pointwise_relation _ (pointwise_relation _ (⊣⊢)) ==> iff) (@Triple Γ δ τ).
     Proof.
       intros P Q pq s s' eq__s R S rs; subst s'.
       split; intro H.
@@ -316,8 +284,8 @@ Module ProgramLogic.
         + exact H.
     Qed.
 
-    Lemma rule_stm_read_register_backwards {Γ δ σ r v f} (Q : Val σ -> CStore Γ -> L) :
-      # f ⦃ lptsreg r v ∗ (lptsreg r v -∗ Q v δ) ⦄
+    Lemma rule_stm_read_register_backwards {Γ δ σ r v} (Q : Val σ -> CStore Γ -> L) :
+      ⦃ lptsreg r v ∗ (lptsreg r v -∗ Q v δ) ⦄
         stm_read_register r ; δ
       ⦃ Q ⦄.
     Proof.
@@ -328,9 +296,9 @@ Module ProgramLogic.
       subst. now iApply "H1".
     Qed.
 
-    Lemma rule_stm_write_register_backwards {Γ δ σ r v f} {e : Exp Γ σ}
+    Lemma rule_stm_write_register_backwards {Γ δ σ r v} {e : Exp Γ σ}
       (Q : Val σ -> CStore Γ -> L) :
-      # f ⦃ lptsreg r v ∗ (lptsreg r (eval e δ) -∗ Q (eval e δ) δ) ⦄
+      ⦃ lptsreg r v ∗ (lptsreg r (eval e δ) -∗ Q (eval e δ) δ) ⦄
         stm_write_register r e ; δ
       ⦃ Q ⦄.
     Proof.
@@ -344,8 +312,7 @@ Module ProgramLogic.
 
     Definition ValidContract {Γ τ} (c : SepContract Γ τ) (body : Stm Γ τ) : Prop :=
       forall (ι : Valuation (sep_contract_logic_variables c)),
-        ∃ (fuel : nat),
-          # fuel ⦃ interpret_contract_precondition c ι ⦄
+          ⦃ interpret_contract_precondition c ι ⦄
             body ; inst_contract_localstore c ι
           ⦃ fun v _ => interpret_contract_postcondition c ι v ⦄.
 
@@ -354,20 +321,20 @@ Module ProgramLogic.
         CEnv f = Some c ->
         ValidContract c (FunDef f).
 
-    Definition TValidContract {Γ τ} (fuel : nat) (c : SepContract Γ τ) (body : Stm Γ τ) : Prop :=
+    Definition TValidContract {Γ τ} (c : SepContract Γ τ) (body : Stm Γ τ) : Prop :=
       forall (ι : Valuation (sep_contract_logic_variables c)),
-          # fuel ⦃ interpret_contract_precondition c ι ⦄
+          ⦃ interpret_contract_precondition c ι ⦄
             body ; inst_contract_localstore c ι
           ⦃ fun v _ => interpret_contract_postcondition c ι v ⦄.
 
-    Definition TValidContractCEnv (fuel : nat) : Prop :=
+    Definition TValidContractCEnv : Prop :=
       forall (Δ : PCtx) (τ : Ty) (f : 𝑭 Δ τ) (c : SepContract Δ τ),
         CEnv f = Some c ->
-        TValidContract fuel c (FunDef f).
+        TValidContract c (FunDef f).
 
   End Triples.
 
-  Notation "# f ⦃ P ⦄ s ; δ ⦃ Q ⦄" := (@Triple _ _ _ δ _ f P%I s Q%I) (at level 50).
+  Notation "⦃ P ⦄ s ; δ ⦃ Q ⦄" := (@Triple _ _ _ δ _ P%I s Q%I).
 
 End ProgramLogic.
 End ProgramLogicOn.
